<?xml version="1.0" encoding="UTF-8"?>
<!-- 
	Flow Cytometry - Metadata relations 
	RDF Schema , version 1.0, Josef Spidlen, June 30th 2006
	http://www.flowcyt.org/
	
	Note: this schema is represented in the RDF M&S abbreviated syntax 
	http://www.w3.org/TR/REC-rdf-syntax/#abbreviatedSyntax 
-->
<rdf:RDF xmlns:obo="http://www.aiai.ed.ac.uk/resources/go/obo.owl#" xmlns:rdf="http://www.w3.org/1999/02/22-rdf-syntax-ns#" xmlns:rdfs="http://www.w3.org/2000/01/rdf-schema#">
	<!--  

	Class declarations   

	-->
	<rdfs:Class rdf:ID="fcsdata">
		<rdfs:subClassOf rdf:resource="http://www.aiai.ed.ac.uk/resources/go/obo.owl#ObjectClass"/>
		<rdfs:isDefinedBy rdf:resource="http://www.isac-net.org/std/rdf/meta-relations/1.0/flow#fcsdata"/>
		<rdfs:comment xml:lang="en">Any encapsulation of flow cytometry data, e.g., an FCS data file or an FCS data set.</rdfs:comment>
		<rdfs:label xml:lang="en">FCS Data</rdfs:label>
	</rdfs:Class>
	<rdfs:Class rdf:ID="datafile">
		<rdfs:subClassOf rdf:resource="http://www.isac-net.org/std/rdf/meta-relations/1.0/flow#fcsdata"/>
		<rdfs:isDefinedBy rdf:resource="http://www.isac-net.org/std/rdf/meta-relations/1.0/flow#datafile"/>
		<rdfs:comment xml:lang="en">An FCS data file.</rdfs:comment>
		<rdfs:label xml:lang="en">FCS Data File</rdfs:label>
	</rdfs:Class>
	<rdfs:Class rdf:ID="dataset">
		<rdfs:subClassOf rdf:resource="http://www.isac-net.org/std/rdf/meta-relations/1.0/flow#fcsdata"/>
		<obo:partOf rdf:resource="http://www.isac-net.org/std/rdf/meta-relations/1.0/flow#datafile"/>
		<rdfs:isDefinedBy rdf:resource="http://www.isac-net.org/std/rdf/meta-relations/1.0/flow#dataset"/>
		<rdfs:comment xml:lang="en">An FCS data set. The URI of a dataset is created as a concatenation of the data file URI with the “#” character followed by the number of the data set within the data file. The number of the first data set is 1.</rdfs:comment>
		<rdfs:label xml:lang="en">FCS Data Set</rdfs:label>
	</rdfs:Class>
	<rdfs:Class rdf:ID="gating">
		<rdfs:subClassOf rdf:resource="http://www.aiai.ed.ac.uk/resources/go/obo.owl#ObjectClass"/>
		<rdfs:isDefinedBy rdf:resource="http://www.isac-net.org/std/rdf/meta-relations/1.0/flow#gating"/>
		<rdfs:comment xml:lang="en">Gates assigned to a data file (data set)</rdfs:comment>
		<rdfs:label xml:lang="en">Gating File</rdfs:label>
	</rdfs:Class>
	<rdfs:Class rdf:ID="transformation">
		<rdfs:subClassOf rdf:resource="http://www.aiai.ed.ac.uk/resources/go/obo.owl#ObjectClass"/>
		<rdfs:isDefinedBy rdf:resource="http://www.isac-net.org/std/rdf/meta-relations/1.0/flow#transformation"/>
		<rdfs:comment xml:lang="en">Transformation that was used for processing  the data (e.g., while gating or displaying it)</rdfs:comment>
		<rdfs:label xml:lang="en">Transformation File</rdfs:label>
	</rdfs:Class>
	<rdfs:Class rdf:ID="compensation">
		<rdfs:subClassOf rdf:resource="http://www.aiai.ed.ac.uk/resources/go/obo.owl#ObjectClass"/>
		<rdfs:isDefinedBy rdf:resource="http://www.isac-net.org/std/rdf/meta-relations/1.0/flow#compensation"/>
		<rdfs:comment xml:lang="en">Specification of how to compensate parameters of a data file (data set). To reference a particular compensation (spilloverMatrix element of the compensation description XML file), the URI of the spillover matrix is created as a concatenation of the compensation file URI with the “#” character followed by the value of the id attribute of the spilloverMatrix element.</rdfs:comment>
		<rdfs:label xml:lang="en">Compensation File</rdfs:label>
	</rdfs:Class>
	<!--  

	Property declarations   

	-->
	<rdf:Property rdf:ID="gated_by">
		<rdfs:domain rdf:resource="http://www.isac-net.org/std/rdf/meta-relations/1.0/flow#fcsdata"/>
		<rdfs:range rdf:resource="http://www.isac-net.org/std/rdf/meta-relations/1.0/flow#gating"/>
		<rdfs:isDefinedBy rdf:resource="http://www.isac-net.org/std/rdf/meta-relations/1.0/flow#gated_by"/>
		<rdfs:comment xml:lang="en">Property of being gated (FCS data resource is gated by a gating resource).</rdfs:comment>
		<rdfs:label xml:lang="en">Being gated by</rdfs:label>
	</rdf:Property>
	<rdf:Property rdf:ID="transformed_by">
		<rdfs:domain rdf:resource="http://www.isac-net.org/std/rdf/meta-relations/1.0/flow#fcsdata"/>
		<rdfs:range rdf:resource="http://www.isac-net.org/std/rdf/meta-relations/1.0/flow#transformation"/>
		<rdfs:isDefinedBy rdf:resource="http://www.isac-net.org/std/rdf/meta-relations/1.0/flow#transformed_by"/>
		<rdfs:comment xml:lang="en">Property of being transformed (parameters of an FCS data resource are transformed by a transformation resource).</rdfs:comment>
		<rdfs:label xml:lang="en">Being transformed by</rdfs:label>
	</rdf:Property>
	<rdf:Property rdf:ID="compensated_by">
		<rdfs:domain rdf:resource="http://www.isac-net.org/std/rdf/meta-relations/1.0/flow#fcsdata"/>
		<rdfs:range rdf:resource="http://www.isac-net.org/std/rdf/meta-relations/1.0/flow#compensation"/>
		<rdfs:isDefinedBy rdf:resource="http://www.isac-net.org/std/rdf/meta-relations/1.0/flow#compensated_by"/>
		<rdfs:comment xml:lang="en">Property of being compensated (FCS data resource is compensated by a compensation resource).</rdfs:comment>
		<rdfs:label>Being compensated by</rdfs:label>
	</rdf:Property>
</rdf:RDF>
